fe25519/fe25519_mul_stage12_ands.v
@@ -601,7 +601,7 @@ Definition fe25519_mul_stage12_ands_spec :=
 
 
 From mathcomp Require Import ssreflect eqtype ssrbool.
-From mQhasm Require Import Verify.
+From mQhasm Require Import zVerify.
 
 Lemma valid_fe25519_mul_stage12_ands_spec :
   valid_spec fe25519_mul_stage12_ands_spec.
